nits

experiments/hyper/StRel.fst
@@ -25,11 +25,11 @@ type wst (a:Type) = wp:(wst0 a){wst_monotonic wp}
 unfold let ret_wst (x:'a) : wst 'a = fun p s0 -> p (x,s0)
 unfold let bind_wst (m:wst 'a) (f:'a -> wst 'b) : wst 'b = fun p s0 -> m (fun (x,s1) -> f x p s1) s0
 
-val theta : st 'a -> wst 'a
-let theta m = fun p s0 -> p (m s0)
+val theta_st : st 'a -> wst 'a
+let theta_st m = fun p s0 -> p (m s0)
 
 let lemma_theta_morphism (m:st 'a) (f:'a -> st 'b) : Lemma (
-  forall s0 p. theta (bind_st m f) p s0 <==> bind_wst (theta m) (fun x -> theta (f x)) p s0
+  forall s0 p. theta_st (bind_st m f) p s0 <==> bind_wst (theta_st m) (fun x -> theta_st (f x)) p s0
 ) = ()
 
 (** Relational State Monad **)
@@ -58,6 +58,12 @@ let seq_cont (#a #b:Type) (wf : a -> wstrel b) (p:wstrel_post b) ((x1,s1):a*stat
 unfold let bind_wstrel (#a #b:Type) (wm : wstrel a) (wf : a -> wstrel b) : wstrel b =
   fun p -> wm (seq_cont wf p)
 
+let get_wstrel l : wstrel int = 
+  fun p s0 s1 -> p (s0 l, s0) (s1 l, s1)
+
+let put_wstrel l v : wstrel unit =
+  fun p s0 s1 -> p ((), st_upd s0 l v) ((), st_upd s1 l v)
+
 let (====) #a (w1:wstrel a) (w2:wstrel a) =
   forall p s1 s2 . w1 p s1 s2 <==> w2 p s1 s2
 
@@ -82,26 +88,26 @@ let wstrel_monad_law3 (#a #b #c:Type) (wm:wstrel a) (wf:a -> wstrel b) (wg:b -> 
 unfold let (⊑) (wp1 wp2: wstrel 'a): Type0 =
   forall p s0 s1. wp2 p s0 s1 ==> wp1 p s0 s1
 
-val theta_rel : st 'a -> wstrel 'a
-let theta_rel m =
-  fun p s0 s1 -> theta m (fun r1 -> theta m (p r1) s1) s0
+val theta_strel : st 'a -> wstrel 'a
+let theta_strel m =
+  fun p s0 s1 -> theta_st m (fun r1 -> theta_st m (p r1) s1) s0
 
 let lemma_theta_rel_morphism #a #b (m:st a) (f:a -> st b) : Lemma (
-  forall p s0 s1. theta_rel (bind_st m f) p s0 s1 <==> bind_wstrel (theta_rel m) (fun x -> theta_rel (f x)) p s0 s1
+  forall p s0 s1. theta_strel (bind_st m f) p s0 s1 <==> bind_wstrel (theta_strel m) (fun x -> theta_strel (f x)) p s0 s1
 ) =
-  introduce forall p s0 s1. (theta_rel (bind_st m f) p s0 s1 <==> bind_wstrel (theta_rel m) (fun x -> theta_rel (f x)) p s0 s1)
+  introduce forall p s0 s1. (theta_strel (bind_st m f) p s0 s1 <==> bind_wstrel (theta_strel m) (fun x -> theta_strel (f x)) p s0 s1)
 with begin
      calc (<==>) {
-       theta_rel (bind_st m f) p s0 s1;
+       theta_strel (bind_st m f) p s0 s1;
        <==> { _ by (
-         norm [delta_only [`%theta_rel];zeta];
+         norm [delta_only [`%theta_strel];zeta];
          compute ()) }
-       bind_wstrel (theta_rel m) (fun x -> theta_rel (f x)) p s0 s1;
+       bind_wstrel (theta_strel m) (fun x -> theta_strel (f x)) p s0 s1;
      }
   end
 
 type dm (a:Type) (w:wstrel a) =
-  m:(st a){theta_rel m ⊑ w}
+  m:(st a){theta_strel m ⊑ w}
 
 let ret_dm (a:Type) (x:a) : dm a (ret_wstrel x) = ret_st x
 
@@ -110,21 +116,21 @@ let bind_dm (a:Type) (b:Type)
             (m:dm a wm) (f:(x:a -> dm b (wf x))) :
             dm b (bind_wstrel wm wf) =
   lemma_theta_rel_morphism m f;
-  assert (theta_rel (bind_st m f) ⊑ bind_wstrel (theta_rel m) (fun x -> theta_rel (f x)));
-  assert (theta_rel m ⊑ wm);
-  assert (bind_wstrel (theta_rel m) (fun x -> theta_rel (f x)) ⊑ bind_wstrel wm wf);
-  assert (theta_rel (bind_st m f) ⊑ bind_wstrel wm wf);
+  assert (theta_strel (bind_st m f) ⊑ bind_wstrel (theta_strel m) (fun x -> theta_strel (f x)));
+  assert (theta_strel m ⊑ wm);
+  assert (bind_wstrel (theta_strel m) (fun x -> theta_strel (f x)) ⊑ bind_wstrel wm wf);
+  assert (theta_strel (bind_st m f) ⊑ bind_wstrel wm wf);
   bind_st m f
 
 let subcomp_dm (a:Type) (wp1 wp2:wstrel a) (m : dm a wp1) : Pure (dm a wp2) (requires (wp1  ⊑ wp2)) (ensures (fun _ -> True)) = m
 
 unfold
-let hist_if_then_else (wp1 wp2:wstrel 'a) (b:bool) : wstrel 'a =
+let wstrel_if_then_else (wp1 wp2:wstrel 'a) (b:bool) : wstrel 'a =
   fun p s0 s1 -> (b ==> wp1 p s0 s1) /\ ((~b) ==> wp2 p s0 s1)
 
 let dm_if_then_else (a : Type u#a) 
   (wp1 wp2: wstrel a) (f : dm a wp1) (g : dm a wp2) (b : bool) : Type =
-  dm a (hist_if_then_else wp1 wp2 b)
+  dm a (wstrel_if_then_else wp1 wp2 b)
 
 total
 reifiable
@@ -165,11 +171,11 @@ let get l : StRel int (fun _ _ -> True) (fun is0 is1 (x0,s0) (x1,s1) -> is0 == s
 let put l v : StRel unit (fun _ _ -> True) (fun is0 is1 (_,s0) (_,s1) -> s0 == st_upd is0 l v /\ s1 == st_upd is1 l v) =
   StRelWp?.reflect (st_put l v)
 
-let test () : StRel unit (fun _ _ -> True) (fun _ _ (_,s0) (_,s1) -> s0 false == s1 false) =
+let test () : StRel unit (fun is0 is1 -> is0 false == is1 false) (fun _ _ (_,s0) (_,s1) -> s0 false == s1 false) =
   let x = get true in
   if x = 1 then put false x else put false 1
 
 [@expect_failure]
-let test2 () : StRel unit (fun _ _ -> True) (fun _ _ (_,s0) (_,s1) -> s0 false <> s1 false) =
+let test2 () : StRel unit (fun is0 is1 -> is0 false == is1 false) (fun _ _ (_,s0) (_,s1) -> s0 false <> s1 false) =
   let x = get true in
   if x = 1 then put false x else put false 1
